theories/Lemma.v
@@ -13,21 +13,20 @@ Set Strict Implicit.
 Section lem.
   Variable typ : Type.
   Variable RType_typ : RType typ.
-  Variable expr : Type.
+  Variable expr : tenv typ -> tenv typ -> typ -> Type.
   Variable Expr_expr : Expr _ expr.
   Hypothesis ExprOk_expr : ExprOk Expr_expr.
-  Variable conclusion : Type.
-
-  Record lemma : Type := Build_lemma
-  { vars : list typ
-  ; premises : list expr
-  ; concl : conclusion
-  }.
-
-  Variable conclusionD : forall us vs, conclusion -> ResType us vs Prop.
+  Variable conclusion : tenv typ -> tenv typ -> Type.
+  Variable conclusionD : forall us vs, conclusion us vs -> ResType us vs Prop.
 
   Context {tyProp : typ}.
   Variable Provable' : typD nil tyProp -> Prop.
+
+  Record lemma tus tvs : Type := Build_lemma
+  { vars : list typ
+  ; premises : list (expr tus (vars ++ tvs) tyProp)
+  ; concl : conclusion tus (vars ++ tvs)
+  }.
 
   Fixpoint foralls (ls : list typ) : (hlist (typD nil) ls -> Prop) -> Prop :=
     match ls as ls return (hlist (typD nil) ls -> Prop) -> Prop with
@@ -95,99 +94,6 @@ Section lem.
     rewrite H. rewrite IHForall2; eauto. reflexivity.
   Qed.
 
-  Definition lemmaD' (tus tvs : tenv typ) (l : lemma)
-  : ResType tus tvs Prop :=
-    match
-        Traversable.mapT (T := list) (F := option)
-                         (fun e : expr => exprD' tus (vars l ++ tvs) tyProp e)
-                         (premises l)
-      , conclusionD tus (vars l ++ tvs) (concl l)
-    with
-      | Some prems , Some concl =>
-        Some (fun us vs =>
-                foralls (fun h : hlist (typD nil) (vars l) =>
-                           let vs' := hlist_app h vs in
-                           impls (map (fun x => Provable' (x us vs')) prems)
-                                 (concl us vs')))
-      | _ , _ => None
-    end.
-
-  Hypothesis conclusionD_weakenU
-  : forall tus tvs l lD,
-      conclusionD tus tvs l = Some lD ->
-      forall tus',
-        exists lD',
-          conclusionD (tus ++ tus') tvs l = Some lD' /\
-          forall us us' vs,
-            lD us vs <-> lD' (hlist_app us us') vs.
-  Hypothesis conclusionD_weakenV
-  : forall tus tvs l lD,
-      conclusionD tus tvs l = Some lD ->
-      forall tvs',
-        exists lD',
-          conclusionD tus (tvs ++ tvs') l = Some lD' /\
-          forall us vs vs',
-            lD us vs <-> lD' us (hlist_app vs vs').
-
-  Opaque Traversable.mapT.
-
-  Lemma mapT_compose'
-  : forall (T V : Type)
-           (R : T -> V -> Prop)
-           (f : T -> option V),
-      (forall x a,
-         f x = Some a -> R x a) ->
-      forall (ls : list T) a,
-        mapT f ls = Some a ->
-        Forall2 R ls a.
-  Proof.
-    induction ls.
-    { simpl.
-      intros. rewrite list_mapT_nil in H0.
-      inv_all; subst. constructor. }
-    { intros. rewrite list_mapT_cons in H0.
-      forward. inv_all; subst.
-      specialize (IHls _ eq_refl). apply H in H0.
-      constructor; auto. }
-  Qed.
-
-  Lemma mapT_compose''
-  : forall (T V : Type)
-           (P : T -> Prop)
-           (R : T -> V -> Prop)
-           (f : T -> option V),
-      (forall x, P x -> exists a, f x = Some a /\ R x a) ->
-      forall ls,
-        Forall P ls ->
-        exists ls',
-          mapT f ls = Some ls' /\
-          Forall2 R ls ls'.
-  Proof.
-    clear. induction 2; intros.
-    { exists nil. rewrite list_mapT_nil. eauto. }
-    { eapply H in H0.
-      forward_reason.
-      rewrite list_mapT_cons. rewrite H0. rewrite H2.
-      eauto. }
-  Qed.
-
-  Lemma mapT_success
-  : forall (T V : Type)
-           (P : T -> Prop)
-           (f : T -> option V),
-      (forall x a, f x = Some a -> P x) ->
-      forall ls ls',
-        mapT f ls = Some ls' ->
-        Forall P ls.
-  Proof.
-    clear.
-    induction ls; simpl; intros.
-    { rewrite list_mapT_nil in *. inv_all; subst; auto. }
-    { rewrite list_mapT_cons in *. forward.
-      apply H in H0. inv_all; subst.
-      specialize (IHls _ eq_refl).
-      constructor; auto. }
-  Qed.
 
   Lemma Forall2_map1
   : forall T U V (f : T -> V) (R : V -> U -> Prop)
@@ -217,232 +123,78 @@ Section lem.
       { inversion H. subst. constructor; auto. eapply IHls. eauto. } }
   Qed.
 
-  Lemma lemmaD'_weakenU
-  : forall tus tvs l lD,
-      lemmaD' tus tvs l = Some lD ->
+
+  Definition lemmaD' (tus tvs : tenv typ) (l : lemma tus tvs)
+  : ResType tus tvs Prop :=
+    match
+        Traversable.mapT (T := list) (F := option)
+                         (fun e : expr _ _ tyProp => exprD' tus (vars l ++ tvs) tyProp e)
+                         (premises l)
+      , conclusionD (concl l)
+    with
+      | Some prems , Some concl =>
+        Some (fun us vs =>
+                foralls (fun h : hlist (typD nil) (vars l) =>
+                           let vs' := hlist_app h vs in
+                           impls (map (fun x => Provable' (x us vs')) prems)
+                                 (concl us vs')))
+      | _ , _ => None
+    end.
+
+  Variable concl_weaken : forall tus tvs tus' tvs', conclusion tus tvs -> conclusion (tus ++ tus') (tvs ++ tvs').
+  Variable concl_conv : forall tus tvs tus' tvs', (unit -> tus = tus') -> (unit -> tvs = tvs') ->
+                                                  conclusion tus tvs -> conclusion tus' tvs'.
+  Hypothesis concl_weaken_sound
+  : forall tus tvs tus' tvs' (c : conclusion tus tvs) cD,
+      conclusionD c = Some cD ->
+      exists cD',
+        conclusionD (@concl_weaken tus tvs tus' tvs' c) = Some cD' /\
+        forall us vs us' vs',
+          cD us vs <-> cD' (HList.hlist_app us us') (hlist_app vs vs').
+
+(*
+  Hypothesis conclusionD_weakenU
+  : forall tus tvs (l : conclusion tus tvs) lD,
+      conclusionD l = Some lD ->
       forall tus',
         exists lD',
-          lemmaD' (tus ++ tus') tvs l = Some lD' /\
+          conclusionD (tus ++ tus') tvs l = Some lD' /\
           forall us us' vs,
             lD us vs <-> lD' (hlist_app us us') vs.
-  Proof.
-    unfold lemmaD'; simpl; intros.
-    forward.
-    inv_all; subst.
-    generalize (fun H' =>
-                  @mapT_compose' _ _
-                                 (fun e v =>
-                                    exists v',
-                                      exprD' (tus ++ tus') (vars l ++ tvs) tyProp e = Some v' /\
-                                      forall a b c,
-                                        v a b = v' (hlist_app a c) b)
-                   _
-                   H'
-                   _ _ H).
-    match goal with
-      | |- (?X -> _) -> _ =>
-        let H := fresh in
-        assert (H : X) ;
-          [ | intro XXX; specialize (XXX H) ]
-    end.
-    { simpl. intros.
-      eapply exprD'_weakenU with (tus' := tus') (t := tyProp) in H1;
-        eauto with typeclass_instances. }
-    eapply mapT_success
-    with (P := fun e =>
-                 exists v,
-                   exprD' tus (vars l ++ tvs) tyProp e = Some v) in H.
-    generalize H.
-    eapply mapT_compose''
-      with (R :=
-              fun e v' =>
-                forall v,
-                  exprD' tus (vars l ++ tvs) tyProp e  = Some v ->
-                  forall us vs us',
-                    v us vs = v' (hlist_app us us') vs)in H.
-    destruct H as [ ? [ ? ? ] ].
-    rewrite H.
-    { eapply conclusionD_weakenU with (tus' := tus') in H0.
-      forward_reason.
-      Cases.rewrite_all_goal.
-      eexists; split; eauto. intros.
-      simpl. eapply foralls_iff. intros.
-      eapply impls_iff.
-      { rewrite Forall2_map2. rewrite Forall2_map1.
-        clear H. generalize dependent x. revert H4.
-        induction XXX; inversion 2; subst; auto.
-        inversion H4; clear H4; subst.
-        eapply IHXXX in H9; clear IHXXX; eauto.
-        constructor; auto.
-        forward_reason.
-        generalize H4.
-        eapply H7 in H4; clear H7.
-        rewrite <- H4; clear H4.
-        erewrite H5; clear H5. intros.
-        eapply exprD'_weakenU with (tus' := tus') in H4; eauto.
-        forward_reason. rewrite H4 in *.
-        inv_all; subst. instantiate (1 := us'). rewrite <- H5. reflexivity. }
-      { eapply H3. } }
-    { simpl. intros.
-      destruct H2. generalize H2.
-      eapply exprD'_weakenU with (tus' := tus') in H2; eauto.
-      destruct H2 as [ ? [ ? ? ] ].
-      eexists; split; eauto. intros.
-      rewrite H4 in H5. inv_all; subst. auto. }
-    { eauto. }
-  Qed.
-
-  Lemma lemmaD'_weakenV
+  Hypothesis conclusionD_weakenV
   : forall tus tvs l lD,
-      lemmaD' tus tvs l = Some lD ->
+      conclusionD tus tvs l = Some lD ->
       forall tvs',
         exists lD',
-          lemmaD' tus (tvs ++ tvs') l = Some lD' /\
+          conclusionD tus (tvs ++ tvs') l = Some lD' /\
           forall us vs vs',
             lD us vs <-> lD' us (hlist_app vs vs').
-  Proof.
-    (** TODO: This proof is horrible! **)
-    unfold lemmaD'; simpl; intros.
-    forward.
-    inv_all; subst.
-    generalize (fun H' =>
-                  @mapT_compose' _ _
-                                 (fun e v =>
-                                    exists v',
-                                      exprD' tus (vars l ++ tvs ++ tvs') tyProp e = Some v' /\
-                                      forall a b c d,
-                                        v a (hlist_app b c) = v' a (hlist_app b (hlist_app c d)))
-                   _
-                   H'
-                   _ _ H).
-    match goal with
-      | |- (?X -> _) -> _ =>
-        let H := fresh in
-        assert (H : X) ;
-          [ | intro XXX; specialize (XXX H) ]
-    end.
-    { simpl. intros.
-      eapply exprD'_weakenV with (tvs' := tvs') in H1;
-        eauto with typeclass_instances.
-      forward_reason.
-      erewrite (@exprD'_conv _ _ _ _ tus tus
-                            (vars l ++ tvs ++ tvs')
-                            ((vars l ++ tvs) ++ tvs')
-                             _ _ eq_refl).
-      rewrite H1.
-      instantiate (1 := app_ass_trans (vars l) tvs tvs').
-      exists match app_ass_trans (vars l) tvs tvs' in _ = tvs'
-                   return hlist (typD nil) tus ->
-                          hlist (typD nil) tvs' -> typD nil tyProp
-             with
-               | eq_refl => x0
-             end.
-      split.
-      { clear. revert x0.
-        destruct (app_ass_trans (vars l) tvs tvs'). reflexivity. }
-      { intros. erewrite H2. instantiate (1 := d).
-        rewrite hlist_app_assoc.
-        clear.
-        match goal with
-          | |- _ _ match _ with eq_refl => ?Y end = _ _ ?X =>
-            change Y with X; generalize dependent X
-        end.
-        revert x0.
-        destruct (app_ass_trans (vars l) tvs tvs').
-        simpl. reflexivity. } }
-    eapply mapT_success
-    with (P := fun e =>
-                 exists v,
-                   exprD' tus (vars l ++ tvs) tyProp e = Some v) in H.
-    generalize H.
-    eapply mapT_compose''
-      with (f := fun e : expr => exprD' tus (vars l ++ tvs ++ tvs') tyProp e)
-           (R :=
-              fun e v' =>
-                forall v,
-                  exprD' tus (vars l ++ tvs) tyProp e = Some v ->
-                  forall us vs vs' vs'',
-                    v us (hlist_app vs vs') = v' us  (hlist_app vs (hlist_app vs' vs''))) in H.
-    { destruct H as [ ? [ ? ? ] ].
-      rewrite H.
-      eapply conclusionD_weakenV with (tvs' := tvs') in H0.
-      forward_reason.
-      Cases.rewrite_all_goal.
-      assert (conclusionD tus (vars l ++ tvs ++ tvs') (concl l) =
-              Some match app_ass_trans (vars l) tvs tvs' in _ = tvs
-                         return hlist _ tus -> hlist _ tvs -> Prop
-                   with
-                     | eq_refl => x0
-                   end).
-      { clear - H0.
-        generalize dependent (app_ass_trans (vars l) tvs tvs').
-        generalize dependent ((vars l ++ tvs) ++ tvs').
-        generalize dependent (vars l ++ tvs ++ tvs').
-        intros. subst. assumption. }
-      rewrite H4.
-      intros.
-      eexists; split; eauto. intros.
-      simpl. eapply foralls_iff. intros.
-      eapply impls_iff.
-      { rewrite Forall2_map2. rewrite Forall2_map1.
-        clear H. generalize dependent x. revert H5.
-        clear H4 conclusionD_weakenU conclusionD_weakenV H0.
-        induction XXX; inversion 2; subst; auto.
-        clear H8.
-        inversion H5; clear H5; subst.
-        inversion H2; clear H2; subst.
-        constructor; eauto.
-        forward_reason.
-        generalize H0. eapply H9 in H0; clear H9.
-        rewrite <- H0; clear H0.
-        erewrite H2; clear H2. instantiate (1 := vs').
-        intros. eapply H1 in H0.
-        forward_reason. revert H0. Cases.rewrite_all_goal.
-        intros; inv_all; subst. reflexivity. }
-      { rewrite H3. instantiate (1 := vs').
-        rewrite hlist_app_assoc. unfold eq_sym.
-        generalize (app_ass_trans (vars l) tvs tvs').
-        clear. intros.
-        match goal with
-          | |- _ _ match _ with eq_refl => ?Y end <-> _ _ ?X =>
-            change Y with X; generalize dependent X
-        end. revert x0. destruct e. reflexivity. } }
-    { simpl. intros.
-      destruct H2. generalize H2.
-      eapply exprD'_weakenV with (tvs' := tvs') in H2; eauto.
-      destruct H2 as [ ? [ ? ? ] ].
-      intro. rewrite H4.
-      erewrite exprD'_conv with (pfu := eq_refl) (pfv := app_ass_trans (vars l) tvs tvs').
-      rewrite H2.
-      exists (match
-                 app_ass_trans (vars l) tvs tvs' in (_ = tvs'0)
-                 return hlist _ tus -> hlist _ tvs'0 -> typD nil tyProp
-               with
-                 | eq_refl => x1
-               end).
-      split.
-      { clear. revert x1.
-        destruct (app_ass_trans (vars l) tvs tvs'). reflexivity. }
-      { intros. inv_all; subst.
-        erewrite H3. instantiate (1 := vs'').
-        rewrite hlist_app_assoc.
-        clear. revert x1.
-        generalize dependent (hlist_app vs (hlist_app vs' vs'')).
-        destruct (app_ass_trans (vars l) tvs tvs').
-        reflexivity. } }
-    { eauto. }
-  Qed.
+*)
+
+  Opaque Traversable.mapT.
+
+  Definition lemma_weaken (tus tvs tus' tvs' : tenv typ) (l : lemma tus tvs)
+  : lemma (tus ++ tus') (tvs ++ tvs') :=
+    @Build_lemma (tus ++ tus') (tvs ++ tvs')
+                 l.(vars)
+                 (map (fun e =>
+                         conv (fun _ => eq_refl) (fun _ => app_ass_trans l.(vars) tvs tvs')
+                              (weaken tus' tvs' e))
+                      l.(premises))
+                 (concl_conv (fun _ => eq_refl) (fun _ => app_ass_trans l.(vars) tvs tvs')
+                             (concl_weaken tus' tvs' l.(concl))).
 
   Lemma lemmaD'_weaken
-  : forall tus tvs l lD,
-      lemmaD' tus tvs l = Some lD ->
+  : forall tus tvs (l : lemma tus tvs) lD,
+      lemmaD' l = Some lD ->
       forall tus' tvs',
         exists lD',
-          lemmaD' (tus ++ tus') (tvs ++ tvs') l = Some lD' /\
+          lemmaD' (lemma_weaken tus' tvs' l) = Some lD' /\
           forall us us' vs vs',
             lD us vs <-> lD' (hlist_app us us') (hlist_app vs vs').
   Proof.
     clear. intros.
+(*
     eapply lemmaD'_weakenU with (tus' := tus') in H.
     destruct H as [ ? [ ? ? ] ].
     eapply lemmaD'_weakenV with (tvs' := tvs') in H.
@@ -451,43 +203,7 @@ Section lem.
     intros.
     etransitivity. eapply H0. eapply H1.
   Qed.
-
-  Definition lemmaD (us vs : env nil) (l : lemma) : Prop :=
-    let (tus,us) := split_env us in
-    let (tvs,vs) := split_env vs in
-    match lemmaD' tus tvs l with
-      | None => False
-      | Some P => P us vs
-    end.
-
-  Lemma lemmaD_weakenU
-  : forall us us' vs l,
-      lemmaD us vs l ->
-      lemmaD (us ++ us') vs l.
-  Proof.
-    intros.
-    unfold lemmaD in H. forward.
-    red. rewrite split_env_app.
-    Cases.rewrite_all_goal.
-    forward. inv_all. subst. subst.
-    eapply lemmaD'_weakenU with (tus' := x2) in H1.
-    destruct H1 as [ ? [ ? ? ] ].
-    rewrite H1. apply H4. assumption.
-  Qed.
-
-  Lemma lemmaD_weakenV
-  : forall us vs vs' l,
-      lemmaD us vs l ->
-      lemmaD us (vs ++ vs') l.
-  Proof.
-    intros.
-    unfold lemmaD in H. forward.
-    red. rewrite split_env_app.
-    Cases.rewrite_all_goal.
-    forward. inv_all. subst. subst.
-    eapply lemmaD'_weakenV with (tvs' := x2) in H1.
-    destruct H1 as [ ? [ ? ? ] ].
-    rewrite H1. apply H4. assumption.
-  Qed.
+*)
+  Admitted.
 
 End lem.
