theories/provers/DefaultProver.v
@@ -2,6 +2,7 @@
 Require Import ExtLib.Tactics.
 Require Import MirrorCore.TypesI.
 Require Import MirrorCore.ExprI.
+Require Import MirrorCore.EnvI.
 Require Import MirrorCore.ProverI.
 
 Set Implicit Arguments.
@@ -10,14 +11,15 @@ Set Strict Implicit.
 Section default_prover.
   Context {typ : Type}.
   Context {RType_typ : RType typ}.
-  Variable expr : Type.
+  Variable expr : tenv typ -> tenv typ -> typ -> Type.
   Context {Expr_expr : Expr _ expr}.
   Context {Typ0_Prop : Typ0 _ Prop}.
 
-  Definition DefaultProver : @Prover typ expr :=
-  {| Facts := unit
+  Definition DefaultProver : @Prover typ _ _ expr :=
+  {| Facts := fun _ _ => unit
+   ; Facts_weaken := fun _ _ _ _ t => t
    ; Summarize := fun tus tvs es => tt
-   ; Learn := fun t _ _ _ => t
+   ; Learn := fun _ _ t _ => t
    ; Prove := fun _ _ _ _ => false
    |}.
 
